[< Home](/index.html)



**I.2   Sets**



---

***Exercise 3***
(Proof of Proposition 2.7)

**Proposition 2.7**   Let $\{ A_\alpha\ ;\ \alpha \in \mathsf{A} \}$ and $\{ B_\beta\ ;\ \beta \in \mathsf{B} \}$ be families of subsets of a set $X.$

**(i)** Associativity: 

* $( \bigcap_{\alpha} A_\alpha) \cap ( \bigcap_{\beta} B_\beta ) = \bigcap_{(\alpha, \beta)} A_\alpha \cap B_\beta$ 
* $( \bigcup_{\alpha} A_\alpha ) \cup ( \bigcup_{\beta} B_\beta ) = \bigcup_{(\alpha, \beta)} A_\alpha \cup B_\beta$ 

**Proof** 

* $x \in ( \bigcap_{\alpha} A_\alpha ) \cap ( \bigcap_{\beta} B_\beta )$ $\iff$ $\forall \alpha \in \mathsf{A} \ (x \in A_\alpha)$ $\and$ $\forall \beta \in \mathsf{B}\ (x \in B_\beta)$ $\iff$ $\forall \alpha \in \mathsf{A}\ \forall \beta \in \mathsf{B}\ (x \in A_\alpha \cap B_\beta).$ Hence, $( \bigcap_{\alpha} A_\alpha) \cap ( \bigcap_{\beta} B_\beta ) = \bigcap_{(\alpha, \beta)} A_\alpha \cap B_\beta$
* $x \in ( \bigcup_{\alpha} A_\alpha ) \cup ( \bigcup_{\beta} B_\beta )$ $\iff$ $\exists \alpha \in \mathsf{A} \ (x \in A_\alpha)$ $\or$ $\exists \beta \in \mathsf{B}\ (x \in B_\beta)$ $\iff$ $\exists \alpha \in \mathsf{A}\ \exists \beta \in \mathsf{B}\ (x \in A_\alpha \cup B_\beta).$ Hence, $( \bigcup_{\alpha} A_\alpha) \cup ( \bigcup_{\beta} B_\beta ) = \bigcup_{(\alpha, \beta)} A_\alpha \cup B_\beta$

**(ii)** Distributivity: 

* $( \bigcap_{\alpha} A_\alpha) \cup ( \bigcap_{\beta} B_\beta ) = \bigcap_{(\alpha, \beta)} A_\alpha \cup B_\beta$ 
* $( \bigcup_{\alpha} A_\alpha ) \cap ( \bigcup_{\beta} B_\beta ) = \bigcup_{(\alpha, \beta)} A_\alpha \cap B_\beta$ 

**Proof** 

* $x \in ( \bigcap_{\alpha} A_\alpha ) \cup ( \bigcap_{\beta} B_\beta )$ $\iff$ $\forall \alpha \in \mathsf{A} \ (x \in A_\alpha)$ $\or$ $\forall \beta \in \mathsf{B}\ (x \in B_\beta)$ $\iff$ $\exists \alpha \in \mathsf{A}\ \exists \beta \in \mathsf{B}\ (x \in A_\alpha \cup B_\beta).$ Hence, $( \bigcap_{\alpha} A_\alpha) \cup ( \bigcap_{\beta} B_\beta ) = \bigcap_{(\alpha, \beta)} A_\alpha \cup B_\beta$
* $x \in ( \bigcup_{\alpha} A_\alpha ) \cap ( \bigcup_{\beta} B_\beta )$ $\iff$ $\exists \alpha \in \mathsf{A} \ (x \in A_\alpha)$ $\and$ $\exists \beta \in \mathsf{B}\ (x \in B_\beta)$ $\iff$ $\exists \alpha \in \mathsf{A}\ \exists \beta \in \mathsf{B}\ (x \in A_\alpha \cap B_\beta).$ Hence, $( \bigcup_{\alpha} A_\alpha) \cap ( \bigcup_{\beta} B_\beta ) = \bigcup_{(\alpha, \beta)} A_\alpha \cap B_\beta$

**(iii)** de Morgan's laws: 

* $( \bigcap_{\alpha} A_\alpha)^c = \bigcup_{\alpha} A_\alpha^c$ 
* $( \bigcup_{\alpha} A_\alpha)^c = \bigcap_{\alpha} A_\alpha^c$ 

**Proof** 

* $x \in (\bigcap_{\alpha} A_\alpha)^c$ $\iff$ $(x \in X) \and (x \notin \bigcap_{\alpha} A_\alpha )$ $\iff$ $(x \in X) \and (\exists \alpha \in \mathsf{A} \ x \notin A_\alpha )$ $\iff$ $(\exists \alpha \in \mathsf{A}) ( x \in X \and x \notin A_\alpha )$ $\iff$ $(\exists \alpha \in \mathsf{A}) ( x \in A_\alpha^c )$ $\iff$ $x \in \bigcup_{\alpha} A_\alpha^c$ 
* $x \in (\bigcup_{\alpha} A_\alpha)^c$ $\iff$ $(x \in X) \and (x \notin \bigcup_{\alpha} A_\alpha )$ $\iff$ $(x \in X) \and (\forall \alpha \in \mathsf{A} \ x \notin A_\alpha )$ $\iff$ $(\forall \alpha \in \mathsf{A}) ( x \in X \and x \notin A_\alpha )$ $\iff$ $(\forall \alpha \in \mathsf{A}) ( x \in A_\alpha^c )$ $\iff$ $x \in \bigcap_{\alpha} A_\alpha^c$



---

***Exercise 4***

Since $X$ and $Y$ are non-empty, the statements $u \in X$ and $v \in Y$ are true for some $u$ and $v$. We can then reason as follows:
$$
(u \in X) \and (v \in Y) \Leftrightarrow  (u, v) \in X \times Y \Leftrightarrow \\
\Leftrightarrow (u, v) \in Y \times X \Leftrightarrow (u \in Y) \and (v \in X)
$$
Therefore, $X = Y$.



---

***Exercise 5***

**a)**    $x \in (A^c)^c$ $\Leftrightarrow$ $(x \notin A^c)$ $\Leftrightarrow$ $\neg(x \in A^c)$ $\Leftrightarrow$ 
$\Leftrightarrow$ $\neg(x \notin A)$ $\Leftrightarrow$ $(x \in A).$
Hence, $(A^c)^c = A.$



**b)**    $x \in (A \cap A^c)$ $\Leftrightarrow$ $(x \in A) \and (x \notin A).$ 
Reductio ad absurdum. So the original assumption is false. That is, $x \notin (A \cap A^c).$ Hence, $A \cap A^c = \empty.$ 



**c)**    $x \in (A \cup A^c)$ $\Leftrightarrow$ $(x \in A) \or (x \notin A)$ $\Leftrightarrow$ $x \in X.$ 
The last iff statement is a consequence of the basic logical fact that True $\Leftrightarrow$ True is valid for *any* two True statements. 
Hence, $A \cup A^c = X.$ 



**d)**    $(A^c \cup B) \cap (A \cap B^c)$ $= (A^c \cup B) \cap (B^c \cap A)$ $= ((A^c \cup B) \cap B^c) \cap A$ $= ((A^c \cap B^c) \cup (B \cap B^c)) \cap A$ $= ((A^c \cap B^c) \cup \empty) \cap A$ $= (B^c \cap A^c) \cap A$ $= B^c \cap (A^c \cap A)$ $= (B^c \cap \empty)$ $= \empty.$ 





---

***Exercise 6***

* Proof of the first result:
  $$
  \begin{align*}
  x &\in\!\! \bigcup_{A \in \mathcal{P}(X)}\!\! A \iff \exists A \in \mathcal{P}(X) : x \in A \\
  & \iff x \in X
  \end{align*}
  $$
  
* The following reductio ad absurdum proves the second result
  $$
  \begin{align*}
  x &\in\!\! \bigcap_{A \in \mathcal{P}(X)}\!\! A \iff \forall A \in \mathcal{P}(X) : x \in A \\
  & \iff x \in \empty
  \end{align*}
  $$



[< Home](/index.html)

