[< Home](/index.html)



**I.2   Sets**



---

***Exercise 3***
(Proof of Proposition 2.7)

**Proposition 2.7**   Let $\{ A_\alpha\ ;\ \alpha \in \mathsf{A} \}$ and $\{ B_\beta\ ;\ \beta \in \mathsf{B} \}$ be families of subsets of a set $X.$

**(i)** Associativity: 

* $( \bigcap_{\alpha} A_\alpha) \cap ( \bigcap_{\beta} B_\beta ) = \bigcap_{(\alpha, \beta)} A_\alpha \cap B_\beta$ 
* $( \bigcup_{\alpha} A_\alpha ) \cup ( \bigcup_{\beta} B_\beta ) = \bigcup_{(\alpha, \beta)} A_\alpha \cup B_\beta$ 

**Proof** 

* $x \in ( \bigcap_{\alpha} A_\alpha ) \cap ( \bigcap_{\beta} B_\beta )$ $\iff$ $\forall \alpha \in \mathsf{A} \ (x \in A_\alpha)$ $\and$ $\forall \beta \in \mathsf{B}\ (x \in B_\beta)$ $\iff$ $\forall \alpha \in \mathsf{A}\ \forall \beta \in \mathsf{B}\ (x \in A_\alpha \cap B_\beta).$ Hence, $( \bigcap_{\alpha} A_\alpha) \cap ( \bigcap_{\beta} B_\beta ) = \bigcap_{(\alpha, \beta)} A_\alpha \cap B_\beta.$
* $x \in ( \bigcup_{\alpha} A_\alpha ) \cup ( \bigcup_{\beta} B_\beta )$ $\iff$ $\exists \alpha \in \mathsf{A} \ (x \in A_\alpha)$ $\or$ $\exists \beta \in \mathsf{B}\ (x \in B_\beta)$ $\iff$ $\exists \alpha \in \mathsf{A}\ \exists \beta \in \mathsf{B}\ (x \in A_\alpha \cup B_\beta).$ Hence, $( \bigcup_{\alpha} A_\alpha) \cup ( \bigcup_{\beta} B_\beta ) = \bigcup_{(\alpha, \beta)} A_\alpha \cup B_\beta.$

**(ii)** Distributivity: 

* $( \bigcap_{\alpha} A_\alpha) \cup ( \bigcap_{\beta} B_\beta ) = \bigcap_{(\alpha, \beta)} A_\alpha \cup B_\beta$ 
* $( \bigcup_{\alpha} A_\alpha ) \cap ( \bigcup_{\beta} B_\beta ) = \bigcup_{(\alpha, \beta)} A_\alpha \cap B_\beta$ 

**Proof** 

* $x \in ( \bigcap_{\alpha} A_\alpha ) \cup ( \bigcap_{\beta} B_\beta )$ $\iff$ $\forall \alpha \in \mathsf{A} \ (x \in A_\alpha)$ $\or$ $\forall \beta \in \mathsf{B}\ (x \in B_\beta)$ $\iff$ $\exists \alpha \in \mathsf{A}\ \exists \beta \in \mathsf{B}\ (x \in A_\alpha \cup B_\beta).$ Hence, $( \bigcap_{\alpha} A_\alpha) \cup ( \bigcap_{\beta} B_\beta ) = \bigcap_{(\alpha, \beta)} A_\alpha \cup B_\beta.$
* $x \in ( \bigcup_{\alpha} A_\alpha ) \cap ( \bigcup_{\beta} B_\beta )$ $\iff$ $\exists \alpha \in \mathsf{A} \ (x \in A_\alpha)$ $\and$ $\exists \beta \in \mathsf{B}\ (x \in B_\beta)$ $\iff$ $\exists \alpha \in \mathsf{A}\ \exists \beta \in \mathsf{B}\ (x \in A_\alpha \cap B_\beta).$ Hence, $( \bigcup_{\alpha} A_\alpha) \cap ( \bigcup_{\beta} B_\beta ) = \bigcup_{(\alpha, \beta)} A_\alpha \cap B_\beta.$

**(iii)** de Morgan's laws: 

* $( \bigcap_{\alpha} A_\alpha)^c = \bigcup_{\alpha} A_\alpha^c$ 
* $( \bigcup_{\alpha} A_\alpha)^c = \bigcap_{\alpha} A_\alpha^c$ 

**Proof** 

* $x \in (\bigcap_{\alpha} A_\alpha)^c$ $\iff$ $(x \in X) \and (x \notin \bigcap_{\alpha} A_\alpha )$ $\iff$ $(x \in X) \and (\exists \alpha \in \mathsf{A} \ x \notin A_\alpha )$ $\iff$ $(\exists \alpha \in \mathsf{A}) ( x \in X \and x \notin A_\alpha )$ $\iff$ $(\exists \alpha \in \mathsf{A}) ( x \in A_\alpha^c )$ $\iff$ $x \in \bigcup_{\alpha} A_\alpha^c$ 
* $x \in (\bigcup_{\alpha} A_\alpha)^c$ $\iff$ $(x \in X) \and (x \notin \bigcup_{\alpha} A_\alpha )$ $\iff$ $(x \in X) \and (\forall \alpha \in \mathsf{A} \ x \notin A_\alpha )$ $\iff$ $(\forall \alpha \in \mathsf{A}) ( x \in X \and x \notin A_\alpha )$ $\iff$ $(\forall \alpha \in \mathsf{A}) ( x \in A_\alpha^c )$ $\iff$ $x \in \bigcap_{\alpha} A_\alpha^c$



---

***Exercise 4***

Since $X$ and $Y$ are non-empty, the statements $u \in X$ and $v \in Y$ are true for some $u$ and $v$. We can then reason as follows:
$$
(u \in X) \and (v \in Y) \Leftrightarrow  (u, v) \in X \times Y \Leftrightarrow \\
\Leftrightarrow (u, v) \in Y \times X \Leftrightarrow (u \in Y) \and (v \in X)
$$
Therefore, $X = Y$.



[< Home](/index.html)

