[Home](/index.html)  >  [Zorich Solutions](/vaz-ma/vaz-ma-solutions.html)




**1.2	Sets and Elementary Operations on Them**



---

***Exercise 1***

**a)**	$(A \subset C ) \wedge (B \subset C)$ $\iff$ $\Big( (A \cup B ) \subset C \Big)$

* $(\Rightarrow)$ Assume that LHS is true. By definition of union, $x \in A \cup B$ $\implies$ $(x\in A) \or (x \in B).$ In either case, it follows from LHS, that $x \in C.$ 
* $(\Leftarrow)$ Assume that RHS is true. Now, $x \in A$ $\implies$ $x\in A \cup B$ $\implies$ $x \in C.$ Where, the first implication is true by definition of union, whereas the second implication is true because we assumed that RHS is true. By a similar argument, $x \in B$ $\implies$ $x \in C.$



**b)**    $(C \subset A ) \wedge (C \subset B)$ $\iff$ $\big( C \subset (A \cap B ) \big)$

* $(\Rightarrow)$ Assume that LHS is true. Then, $x \in C$ $\implies$ $(x\in A) \and (x \in B).$ By definition of intersection, it follows that $x \in A \cap B.$ 
* $(\Leftarrow)$ Assume that RHS is true. Now, $x \in C$ $\implies$ $x\in A \cap B$ $\implies$ $x \in A.$ Where, the first implication is true because we assumed that RHS is true, whereas the second implication is true by definition of intersection. By a similar argument, $x \in C$ $\implies$ $x \in B.$



**c)**    $ C_M \big( C_MA \big) = A $

$x \in C_M(C_M A)$ $\iff$ $(x \notin C_M A) $ $\iff$ $x \in A.$ 



**d)**    $(A \subset C_MB )$ $\iff$ $(B \subset C_MA )$

$\big( A \subset C_MB \big)$ $\iff$ $(x \in A \Rightarrow x \in C_MB )$ $\iff$ $\big( (x \in A) \Rightarrow (x \notin B) \big)$ $\iff$ $\big( (x \in B) \Rightarrow (x \notin A) \big)$ $\iff$ $\big( (x \in B) \Rightarrow (x \in C_MA)  \big)$  $\iff$ $\big( B \subset C_MA  \big).$ In the third equivalence statement, we have made use of the fact that the implication $P \Rightarrow Q$ is equivalent to its contrapositive: $\neg Q \Rightarrow \neg P.$



**e)**    $(A \subset B )$ $\iff$ $(C_MA \supset C_MB )$

$\big( A \subset B \big)$ $\iff$ $\big( x \in A \Rightarrow x \in B \big)$ $\iff$ $\big(  (x \notin B) \Rightarrow (x \notin A) \big)$ $\iff$ $\big( (x \in C_MB) \Rightarrow (x \in C_MA) \big)$ $\iff$ $\big( C_MB \subset C_MA  \big)$ $\iff$ $\big( C_MA \supset C_MB  \big).$




---

***Exercise 2***

(a) and (b) state respectively, that the set union and set intersection are associative. The proofs implicitly use the associativity of the logical OR and logical AND operators respectively. (c) states that the set intersection distributes over the set union. Here, the proof implicitly uses the fact that the logical AND distributes over the logical OR operator. Similarly, (d) states that the set union distributes over the set intersection and the proof implicitly uses the fact that the logical OR distributes over the logical AND operator. The proofs merely require mechanical operations with the logical operations and set operations. (a) is solved below as an example.

**a)**	$ A \cup (B \cup C)$ $=$ $(A \cup B ) \cup C$ $:=$ $A \cup B \cup C $

$x \in A \cup (B \cup C)$ $\Leftrightarrow$ $(x \in A) \or (x \in (B \cup C))$ $\Leftrightarrow$ $(x \in A) \or ((x \in B) \or (x \in C))$ $\Leftrightarrow$ $((x \in A) \or (x \in B)) \or (x \in C)$ $\Leftrightarrow$ $(x \in A \cup B) \or (x \in C)$ $\Leftrightarrow$ $x \in (A \cup B) \cup C.$




---

***Exercise 3***

**De Morgan's laws for set operations**. Proofs are elementary as seen below.

**a)**	$ C_M (A \cup B) = C_MA \cap C_MB $

$x \in C_M (A \cup B)$ $\Leftrightarrow$ $x \notin (A \cup B)$ $\Leftrightarrow$ $(x \notin A) \and (x \notin B)$ $\Leftrightarrow$ $(x \in C_M A) \and (x \in C_M B)$ $\Leftrightarrow$ $x \in (C_M A \cap C_M B).$

Note that the second equivalence statement above follows from the fact that $x \notin P$ $:\Leftrightarrow$ $\neg(x \in P),$ along with De Morgan's laws for logical operations proved in the previous section.

**b)**	$ C_M (A \cap B) = C_MA \cup C_MB $

Proof is similar to (a).



---


***Exercise 4***
(Proof of Proposition 2.7)

**Proposition 2.7**   Let $\{ A_\alpha\ ;\ \alpha \in \mathsf{A} \}$ and $\{ B_\beta\ ;\ \beta \in \mathsf{B} \}$ be families of subsets of a set $X.$

**(i)** Associativity: 

* $( \bigcap_{\alpha} A_\alpha) \cap ( \bigcap_{\beta} B_\beta ) = \bigcap_{(\alpha, \beta)} A_\alpha \cap B_\beta$ 
* $( \bigcup_{\alpha} A_\alpha ) \cup ( \bigcup_{\beta} B_\beta ) = \bigcup_{(\alpha, \beta)} A_\alpha \cup B_\beta$ 

**Proof** 

* $x \in ( \bigcap_{\alpha} A_\alpha ) \cap ( \bigcap_{\beta} B_\beta )$ $\iff$ $\forall \alpha \in \mathsf{A} \ (x \in A_\alpha)$ $\and$ $\forall \beta \in \mathsf{B}\ (x \in B_\beta)$ $\iff$ $\forall \alpha \in \mathsf{A}\ \forall \beta \in \mathsf{B}\ (x \in A_\alpha \cap B_\beta).$ Hence, $( \bigcap_{\alpha} A_\alpha) \cap ( \bigcap_{\beta} B_\beta ) = \bigcap_{(\alpha, \beta)} A_\alpha \cap B_\beta$
* $x \in ( \bigcup_{\alpha} A_\alpha ) \cup ( \bigcup_{\beta} B_\beta )$ $\iff$ $\exists \alpha \in \mathsf{A} \ (x \in A_\alpha)$ $\or$ $\exists \beta \in \mathsf{B}\ (x \in B_\beta)$ $\iff$ $\exists \alpha \in \mathsf{A}\ \exists \beta \in \mathsf{B}\ (x \in A_\alpha \cup B_\beta).$ Hence, $( \bigcup_{\alpha} A_\alpha) \cup ( \bigcup_{\beta} B_\beta ) = \bigcup_{(\alpha, \beta)} A_\alpha \cup B_\beta$

**(ii)** Distributivity: 

* $( \bigcap_{\alpha} A_\alpha) \cup ( \bigcap_{\beta} B_\beta ) = \bigcap_{(\alpha, \beta)} A_\alpha \cup B_\beta$ 
* $( \bigcup_{\alpha} A_\alpha ) \cap ( \bigcup_{\beta} B_\beta ) = \bigcup_{(\alpha, \beta)} A_\alpha \cap B_\beta$ 

**Proof** 

* $x \in ( \bigcap_{\alpha} A_\alpha ) \cup ( \bigcap_{\beta} B_\beta )$ $\iff$ $\forall \alpha \in \mathsf{A} \ (x \in A_\alpha)$ $\or$ $\forall \beta \in \mathsf{B}\ (x \in B_\beta)$ $\iff$ $\exists \alpha \in \mathsf{A}\ \exists \beta \in \mathsf{B}\ (x \in A_\alpha \cup B_\beta).$ Hence, $( \bigcap_{\alpha} A_\alpha) \cup ( \bigcap_{\beta} B_\beta ) = \bigcap_{(\alpha, \beta)} A_\alpha \cup B_\beta$
* $x \in ( \bigcup_{\alpha} A_\alpha ) \cap ( \bigcup_{\beta} B_\beta )$ $\iff$ $\exists \alpha \in \mathsf{A} \ (x \in A_\alpha)$ $\and$ $\exists \beta \in \mathsf{B}\ (x \in B_\beta)$ $\iff$ $\exists \alpha \in \mathsf{A}\ \exists \beta \in \mathsf{B}\ (x \in A_\alpha \cap B_\beta).$ Hence, $( \bigcup_{\alpha} A_\alpha) \cap ( \bigcup_{\beta} B_\beta ) = \bigcup_{(\alpha, \beta)} A_\alpha \cap B_\beta$

**(iii)** de Morgan's laws: 

* $( \bigcap_{\alpha} A_\alpha)^c = \bigcup_{\alpha} A_\alpha^c$ 
* $( \bigcup_{\alpha} A_\alpha)^c = \bigcap_{\alpha} A_\alpha^c$ 

**Proof** 

* $x \in (\bigcap_{\alpha} A_\alpha)^c$ $\iff$ $(x \in X) \and (x \notin \bigcap_{\alpha} A_\alpha )$ $\iff$ $(x \in X) \and (\exists \alpha \in \mathsf{A} \ x \notin A_\alpha )$ $\iff$ $(\exists \alpha \in \mathsf{A}) ( x \in X \and x \notin A_\alpha )$ $\iff$ $(\exists \alpha \in \mathsf{A}) ( x \in A_\alpha^c )$ $\iff$ $x \in \bigcup_{\alpha} A_\alpha^c$ 
* $x \in (\bigcup_{\alpha} A_\alpha)^c$ $\iff$ $(x \in X) \and (x \notin \bigcup_{\alpha} A_\alpha )$ $\iff$ $(x \in X) \and (\forall \alpha \in \mathsf{A} \ x \notin A_\alpha )$ $\iff$ $(\forall \alpha \in \mathsf{A}) ( x \in X \and x \notin A_\alpha )$ $\iff$ $(\forall \alpha \in \mathsf{A}) ( x \in A_\alpha^c )$ $\iff$ $x \in \bigcap_{\alpha} A_\alpha^c$



---

***Exercise 4***

Since $X$ and $Y$ are non-empty, the statements $u \in X$ and $v \in Y$ are true for some $u$ and $v$. We can then reason as follows:
$$
(u \in X) \and (v \in Y) \Leftrightarrow  (u, v) \in X \times Y \Leftrightarrow \\
\Leftrightarrow (u, v) \in Y \times X \Leftrightarrow (u \in Y) \and (v \in X)
$$
Therefore, $X = Y$.



---

***Exercise 5***

**a)**    $x \in (A^c)^c$ $\Leftrightarrow$ $(x \notin A^c)$ $\Leftrightarrow$ $\neg(x \in A^c)$ $\Leftrightarrow$ 
$\Leftrightarrow$ $\neg(x \notin A)$ $\Leftrightarrow$ $(x \in A).$
Hence, $(A^c)^c = A.$



**b)**    $x \in (A \cap A^c)$ $\Leftrightarrow$ $(x \in A) \and (x \notin A).$ 
Reductio ad absurdum. So the original assumption is false. That is, $x \notin (A \cap A^c).$ Hence, $A \cap A^c = \empty.$ 



**c)**    $x \in (A \cup A^c)$ $\Leftrightarrow$ $(x \in A) \or (x \notin A)$ $\Leftrightarrow$ $x \in X.$ 
The last iff statement is a consequence of the basic logical fact that True $\Leftrightarrow$ True is valid for *any* two True statements. 
Hence, $A \cup A^c = X.$ 



**d)**    $(A^c \cup B) \cap (A \cap B^c)$ $= (A^c \cup B) \cap (B^c \cap A)$ $= ((A^c \cup B) \cap B^c) \cap A$ $= ((A^c \cap B^c) \cup (B \cap B^c)) \cap A$ $= ((A^c \cap B^c) \cup \empty) \cap A$ $= (B^c \cap A^c) \cap A$ $= B^c \cap (A^c \cap A)$ $= (B^c \cap \empty)$ $= \empty.$ 





---

***Exercise 6***

* Proof of the first result:
  $$
  \begin{align*}
  x &\in\!\! \bigcup_{A \in \mathcal{P}(X)}\!\! A \iff \exists A \in \mathcal{P}(X) : x \in A \\
  & \iff x \in X
  \end{align*}
  $$
  
* The following reductio ad absurdum proves the second result
  $$
  \begin{align*}
  x &\in\!\! \bigcap_{A \in \mathcal{P}(X)}\!\! A \iff \forall A \in \mathcal{P}(X) : x \in A \\
  & \iff x \in \empty
  \end{align*}
  $$



---

***Exercise 7***

**a)**    $A \times B \ne \empty$  $\Leftrightarrow$  $(A \ne \empty) \and (B \ne \empty)$

* $(\Rightarrow)$ Suppose that  $A \times B \subseteq X \times Y.$ We can now reason as follows: $(a \in A) \and (b \in B)$ $\Leftrightarrow$ $(a,b) \in A \times B$ $\Rightarrow$ $(a,b) \in X \times Y$ $\Rightarrow$ $(a \in X) \and (b \in X)$
  Hence, $(A \subseteq X) \and (B \subseteq Y)$ 
* $(\Leftarrow)$ Suppose that  $(A \subseteq X) \and (B \subseteq Y).$ We can now reason as follows: $(a,b) \in A \times B$ $\Leftrightarrow$ $(a \in A) \and (b \in B)$ $\Rightarrow$ $(a \in X) \and (b \in Y)$ $\Rightarrow$ $(a,b) \in X \times Y$ 
  Hence, $A \times B \subseteq X \times Y$ 

**d)**    $(x,y) \in (X \times Y) \setminus(A\times B) $ $\Leftrightarrow$ $(x,y) \in (X \times Y) \and (x,y) \notin (A\times B) $ $\Leftrightarrow$ $((x \in X) \and (y \in Y)) \and (x \notin A \or y \notin B)$ $\Leftrightarrow$ $((x \in X) \and (y \in Y) \and x \notin A)$ $\or$ $((x \in X) \and (y \in Y) \and y \notin B)$ $\Leftrightarrow$ $((x \in X\setminus A) \and (y \in Y))$ $\or$ $((x \in X) \and (y \in Y\setminus B))$ $\Leftrightarrow$ $((x,y) \in (X\setminus A) \times Y))$ $\or$ $((x,y) \in X \times (Y\setminus B))$ $\Leftrightarrow$ $(x,y) \in ((X\setminus A) \times Y) \cup (X \times (Y\setminus B))$



---

***Exercise 8***

Let $\{ A_\alpha\ ;\ \alpha \in \mathsf{A} \}$ and $\{ B_\beta\ ;\ \beta \in \mathsf{B} \}$ be families of subsets of a set.

**a)**    $(x,y) \in ( \bigcap_{\alpha} A_\alpha ) \times ( \bigcap_{\beta} B_\beta )$ $\iff$ $\forall \alpha \in \mathsf{A} \ (x \in A_\alpha)$ $\and$ $\forall \beta \in \mathsf{B}\ (x \in B_\beta)$ $\iff$ $\forall \alpha \in \mathsf{A}\ \forall \beta \in \mathsf{B}\ ((x,y) \in A_\alpha \times B_\beta)$ 
Hence, $( \bigcap_{\alpha} A_\alpha) \times ( \bigcap_{\beta} B_\beta ) = \bigcap_{(\alpha, \beta)} A_\alpha \times B_\beta$ 

**b)**    $(x,y) \in ( \bigcup_{\alpha} A_\alpha ) \times ( \bigcup_{\beta} B_\beta )$ $\iff$ $\exists \alpha \in \mathsf{A} \ (x \in A_\alpha)$ $\and$ $\exists \beta \in \mathsf{B}\ (x \in B_\beta)$ $\iff$ $\exists \alpha \in \mathsf{A}\ \exists \beta \in \mathsf{B}\ ((x,y) \in A_\alpha \times B_\beta)$ 
Hence, $( \bigcup_{\alpha} A_\alpha) \times ( \bigcup_{\beta} B_\beta ) = \bigcup_{(\alpha, \beta)} A_\alpha \times B_\beta$



[< Zorich Solutions](/vaz-ma/vaz-ma-solutions.html)
